Struct/Struct.lean
@@ -1,6 +1,6 @@
 import Lean
 
-import Struct.Helpers
+-- import Struct.Helpers
 import Struct.CustomTactics
 
 open 
@@ -20,78 +20,6 @@ set_option pp.rawOnError true
   # Description of this file ..
 
 -/
-
-structure StateDiff where
-  newlyChangedGoal : Option Term
-  newDecls : Array LocalDecl -- TODO: Change LocalDecl to something that can't change
-  changedDecls : Array LocalDecl
-  removedDecls : Array LocalDecl
-
-def StateDiff.toMessageData (s : StateDiff) : MessageData :=
-  m!"isGoalChanged: {if s.newlyChangedGoal == none then "false" else "true"}, 
-      newDecls: [{s.newDecls.map fun ldecl => ldecl.type}], 
-      changedDecls: [{s.changedDecls.map fun ldecl => ldecl.type}],
-      removedDecls: [ {s.removedDecls.map fun ldecl => ldecl.type} ]"
-
-def goalsToStateDiff (oldGoal : MVarId) (newGoal : MVarId) : TacticM StateDiff := do
-  let oldGoalType ← instantiateMVars (← oldGoal.getDecl).type
-  let newGoalType ← instantiateMVars (← newGoal.getDecl).type
-  let isSameGoal := oldGoalType.consumeMData == newGoalType.consumeMData
-  let newlyChangedGoal := if isSameGoal then none else some (← delab newGoalType)
-
-  let oldLCtx := (← oldGoal.getDecl).lctx
-  let newLCtx := (← newGoal.getDecl).lctx
-
-  let mut newDecls := #[]
-  let mut changedDecls := #[]
-  let mut removedDecls := #[]
-
-  for newDecl in newLCtx do
-    if !newDecl.isAuxDecl then
-      let mut foundMatch : Bool := false
-      for oldDecl in oldLCtx do
-        if !oldDecl.isAuxDecl then
-          if newDecl.userName == oldDecl.userName then
-            foundMatch := true
-            if !(newDecl.type.consumeMData == oldDecl.type.consumeMData) then
-              changedDecls := changedDecls.push newDecl
-      if !foundMatch then
-        newDecls := newDecls.push newDecl
-
-  for oldDecl in oldLCtx do
-    if !oldDecl.isAuxDecl then
-      let mut foundMatch : Bool := false
-      for newDecl in newLCtx do
-        if !newDecl.isAuxDecl then
-          if oldDecl.userName == newDecl.userName then
-            foundMatch := true
-      if !foundMatch then
-        removedDecls := removedDecls.push oldDecl
-
-  return StateDiff.mk newlyChangedGoal newDecls changedDecls removedDecls
-
--- ## Helpers ..
-def getTacs (ts : TSyntax ``tacticSeq) : TermElabM (Array (TSyntax `tactic)) :=
-  match ts with
-  | `(tacticSeq| { $[$tacs:tactic $[;]?]* }) => return tacs
-  | `(tacticSeq| $[$tacs:tactic $[;]?]*) => return tacs
-  | _ => throwError "unknown syntax"
-
--- TODO REMOVE
-def getUniqueIdent : TermElabM (TSyntax `ident) := do
-  return mkIdent "tmp0"
-
--- TODO REMOVE
-def getIdentWithSuggestion (suggestion : name) : TermElabM (TSyntax `ident) := do
-  return mkIdent "tmp"
-
-def replaceSkipWithNote (old : TSyntax ``inductionAlt) (note : TSyntax `tactic) : TermElabM (TSyntax ``inductionAlt) := do
-  match old with
-  | `(inductionAlt| | $lhs $[$ids]* => skip) => return ← `(inductionAlt| | $lhs $[$ids]* => 
-    $note:tactic
-    sorry)
-  | _ => 
-    throwError "Shouldnt reach"
 
 -- ## State to tactic(Seq) builders
 def mkShow (newGoalTerm : Term) (tacSeq : TSyntax ``tacticSeq) : TermElabM (TSyntax `tactic) := do
@@ -130,21 +58,101 @@ def mkNote (decls : Array LocalDecl := #[]) (optGoal : Option Term := none) (opt
         `(tactic|note $[$binders]*)
 
 
--- TODO Restructure
--- def mkCasesMatch
--- def mkInductionMatch
+-- ## Segment description
+structure StateDiff where
+  newlyChangedGoal : Option Term
+  newDecls : Array LocalDecl
+  changedDecls : Array LocalDecl
+  removedDecls : Array LocalDecl
 
-def mkCases (x : TSyntax ``casesTarget) (y : TSyntax ``binderIdent) : TermElabM (TSyntax ``tacticSeq) := do
-  `(tacticSeq|
-    cases $x
-    case $y =>
-      rfl)
+def StateDiff.toMessageData (s : StateDiff) : MessageData :=
+  m!"isGoalChanged: {if s.newlyChangedGoal == none then "false" else "true"}, 
+      newDecls: [{s.newDecls.map fun ldecl => ldecl.type}], 
+      changedDecls: [{s.changedDecls.map fun ldecl => ldecl.type}],
+      removedDecls: [ {s.removedDecls.map fun ldecl => ldecl.type} ]"
 
--- def mkCase
--- def mkDefaultCases
+def goalsToStateDiff (oldGoal : MVarId) (newGoal : MVarId) : TacticM StateDiff := do
+  let oldGoalType ← instantiateMVars (← oldGoal.getDecl).type
+  let newGoalType ← instantiateMVars (← newGoal.getDecl).type
+  let isSameGoal := oldGoalType.consumeMData == newGoalType.consumeMData
+  let newlyChangedGoal := if isSameGoal then none else some (← delab newGoalType)
+
+  let oldLCtx := (← oldGoal.getDecl).lctx
+  let newLCtx := (← newGoal.getDecl).lctx
+
+  let mut newDecls := #[]
+  let mut changedDecls := #[]
+  let mut removedDecls := #[]
+
+  for newDecl in newLCtx do
+    if !newDecl.isAuxDecl then -- todo isImplementationDetail
+      let mut foundMatch : Bool := false
+      for oldDecl in oldLCtx do
+        if !oldDecl.isAuxDecl then
+          if newDecl.userName == oldDecl.userName then
+            foundMatch := true
+            if !(newDecl.type.consumeMData == oldDecl.type.consumeMData) then
+              changedDecls := changedDecls.push newDecl
+      if !foundMatch then
+        newDecls := newDecls.push newDecl
+
+  for oldDecl in oldLCtx do
+    if !oldDecl.isAuxDecl then
+      let mut foundMatch : Bool := false
+      for newDecl in newLCtx do
+        if !newDecl.isAuxDecl then
+          if oldDecl.userName == newDecl.userName then
+            foundMatch := true
+      if !foundMatch then
+        removedDecls := removedDecls.push oldDecl
+
+  return StateDiff.mk newlyChangedGoal newDecls changedDecls removedDecls
+
+def mapMVarToNote (oldGoal : MVarId) (newGoal : MVarId) : TacticM (TSyntax `tactic) := do
+  newGoal.withContext do
+    let s ← goalsToStateDiff oldGoal newGoal
+    mkNote (s.changedDecls ++ s.newDecls) s.newlyChangedGoal none
+
+def getNotesFromTac (oldGoal : MVarId) (tac : TSyntax `tactic) : TacticM (List (TSyntax `tactic)) := do
+  oldGoal.withContext do
+    withoutModifyingState do 
+      evalTactic tac
+      let mvars ← getUnsolvedGoals
+      mvars.mapM (fun mvar => do mapMVarToNote oldGoal mvar)
+
+def getNotesFromTacSeq (oldGoal : MVarId) (tac : TSyntax ``tacticSeq) : TacticM (List (TSyntax `tactic)) := do
+  oldGoal.withContext do
+    withoutModifyingState do 
+      evalTactic tac
+      let mvars ← getUnsolvedGoals
+      mvars.mapM (fun mvar => do mapMVarToNote oldGoal mvar)
+
+def getTacs (ts : TSyntax ``tacticSeq) : TermElabM (Array (TSyntax `tactic)) :=
+  match ts with
+  | `(tacticSeq| { $[$tacs:tactic]* }) => return tacs
+  | `(tacticSeq| $[$tacs:tactic]*) => return tacs
+  | _ => throwError "unknown syntax"
+
+def replaceHoleWithNoteInductionAlt (old : TSyntax ``inductionAlt) (note : TSyntax `tactic) : TermElabM (TSyntax ``inductionAlt) := do
+  match old with
+  | `(inductionAlt| | $lhs $[$ids]* => ?_) => 
+      `(inductionAlt| | $lhs $[$ids]* => 
+        $note:tactic)
+  | _ => 
+    throwError "Shouldnt reach"
+
+def replaceHoleWithNoteCaseTactic (old : TSyntax `tactic) (note : TSyntax `tactic) : TermElabM (TSyntax `tactic) := do
+  match old with
+  | `(tactic|case $tag $[$ids]* => skip) => 
+      `(tactic|case $tag $[$ids]* => 
+        $note:tactic)
+  | _ => 
+    throwError "Shouldnt reach"
+
 
 -- ## Structured branches
 def structuredIntros (tacSeq : TSyntax ``tacticSeq) (oldGoal : MVarId) : TacticM Unit := do
+  addTrace `xx m!"Testxx"
   evalTactic tacSeq
   match (← getUnsolvedGoals) with
   | [] => throwError "Finishing with intros should be impossible"
@@ -159,9 +167,6 @@ def structuredIntros (tacSeq : TSyntax ``tacticSeq) (oldGoal : MVarId) : TacticM
   | _ => throwError "Unexpected state: Multiple goals after executing intro statement"
 
 -- TODO : Refactor out stuff
--- def mkInductionAlt (goal : MVarId) (target : TSyntax `term) (cInfo : Option ConstantInfo) : TacticM (TSyntax ``inductionAlt) := 
---   goal.withContext do 
---     return (← `(inductionAlt| | $target => skip))
 
 def structuredCasesOrInduction (tacSeq : TSyntax ``tacticSeq) (oldGoal : MVarId) (target : TSyntax `term) (isInduction : Bool) : TacticM Unit :=
   oldGoal.withContext do
@@ -211,7 +216,7 @@ def structuredCasesOrInduction (tacSeq : TSyntax ``tacticSeq) (oldGoal : MVarId)
                   indArgs := indArgs.push (mkIdent indName)
             
             -- TODO consider ?_ instead of skip
-            let case ← `(inductionAlt| | $ctorIdent $[$ctorArgs]* $[$indArgs]* => skip)
+            let case ← `(inductionAlt| | $ctorIdent $[$ctorArgs]* $[$indArgs]* => ?_)
             cases := cases.push case
 
           | _ => addTrace `xx m!"Unexpected state 02"
@@ -223,14 +228,14 @@ def structuredCasesOrInduction (tacSeq : TSyntax ``tacticSeq) (oldGoal : MVarId)
       match isInduction with
       | true => 
         let matchWithoutNotes ← `(tactic| induction $target:term with $[$cases]*)
-        let notes ← InductionHelper.getMVarsFromMatch oldGoal matchWithoutNotes isInduction
-        let casesWithNotes ← cases.zip notes |>.mapM (fun (case, note) => do replaceSkipWithNote case note)
+        let notes ← getNotesFromTac oldGoal matchWithoutNotes
+        let casesWithNotes ← cases.zip notes.toArray |>.mapM (fun (case, note) => do replaceHoleWithNoteInductionAlt case note)
         let matchWithNotes ← `(tactic| induction $target:term with $[$casesWithNotes]*)
         addTrace `test m!"Try this: {matchWithNotes}"
       | false => 
         let matchWithoutNotes ← `(tactic| cases $target:term with $[$cases]*)
-        let notes ← InductionHelper.getMVarsFromMatch oldGoal matchWithoutNotes isInduction
-        let casesWithNotes ← cases.zip notes |>.mapM (fun (case, note) => do replaceSkipWithNote case note)
+        let notes ← getNotesFromTac oldGoal matchWithoutNotes
+        let casesWithNotes ← cases.zip notes.toArray |>.mapM (fun (case, note) => do replaceHoleWithNoteInductionAlt case note)
         let matchWithNotes ← `(tactic| cases $target:term with $[$casesWithNotes]*)
         addTrace `test m!"Try this: {matchWithNotes}"
     | _ => addTrace `xx m!"Unexpected state 00"
@@ -244,8 +249,7 @@ def structureCasesDefault (tacSeq : TSyntax ``tacticSeq) (oldGoal : MVarId) (new
   for newGoal in newGoals do 
     let s ← goalsToStateDiff oldGoal newGoal
 
-    -- Detect inaccessible local context, add to case statement
-    -- For each decl in s.newDecls that hasMacroScopes
+    -- For any inaccessible decl, create a new unused name, and use that
     let mut caseArgs : Array (TSyntax ``binderIdent) := #[]
     for decl in s.newDecls do
       if decl.userName.hasMacroScopes then
@@ -253,20 +257,21 @@ def structureCasesDefault (tacSeq : TSyntax ``tacticSeq) (oldGoal : MVarId) (new
         let caseArgIdent := mkIdent caseArgName
         caseArgs := caseArgs.push (← `(binderIdent|$caseArgIdent:ident))
 
-    -- Construct change annotation
-    -- TODO: Use above caseArg names in this annotation
-    let annotation ← mkNote (s.newDecls ++ s.changedDecls) s.newlyChangedGoal none
-
     -- Construct full case
     let caseIdName := mkIdent (← newGoal.getTag)
     let caseBinderId : TSyntax ``binderIdent ← `(binderIdent|$caseIdName:ident)
-    let case ← `(tactic|case $caseBinderId $[$caseArgs]* => 
-      $annotation:tactic
-      sorry)
+    let case ← `(tactic|case $caseBinderId $[$caseArgs]* => skip)
     cases := cases.push case  
   
+  -- Construct notes with decided names
+  let casesWithoutNotes ← `(tacticSeq| $[$cases]*)
+  let notes ← getNotesFromTacSeq oldGoal casesWithoutNotes
+  let casesWithNotes ← cases.zip notes.toArray |>.mapM (fun (case, note) => do replaceHoleWithNoteCaseTactic case note)
+
+  addTrace `xx m!"Test: {casesWithoutNotes} {casesWithNotes}"
+
   -- Append all 
-  let suggestion ← mkTacticSeqAppendTacs tacSeq cases
+  let suggestion ← mkTacticSeqAppendTacs tacSeq casesWithNotes
   addTrace `structured m!"Try this: {suggestion}"
 
 def structuredDefault (tacSeq : TSyntax ``tacticSeq) (oldGoal : MVarId) : TacticM Unit := do
@@ -319,10 +324,12 @@ def structuredCore (tacSeq : TSyntax ``tacticSeq) : TacticM Unit := do
         => 
         addTrace `structured m!"This tactic is already structured"
         evalTactic tacSeq
-      -- TODO: Currently also matches on patterns, probably wrong matching here
-      | `(tactic|intro $ids:ident*)
-      | `(tactic|intros $ids*)
+      -- TODO: Only match on intro $_, then unpack the content further in structuredIntros
+      | `(tactic|intro $[$ids:ident]*)
+      -- | `(tactic|intros $ids*)
         => 
+        let ids : Array (TSyntax `ident) := ids -- TODO mwe Zulip
+        addTrace `xx m!"{ids.map (fun x => repr x.raw)}"
         structuredIntros tacSeq goal
       | `(tactic|cases $target:term) 
         => structuredCasesOrInduction tacSeq goal target false
@@ -341,117 +348,18 @@ elab &"structured " t:tacticSeq : tactic =>
 
 -- TMP Testing code below
 
-example : α → β → α := by  
-  -- structured intro
-  -- structured intro ha _
-  -- structured intro (ha : α) (_ : β)
-  -- structured intros
-  -- structured intros ha _
-
-  -- TODO: we actually don't want to match on intro patterns, but it still seems to
-  structured intro (ha : α) (_ : β)
-  -- fix (ha : α) (_ : β) ⊢ α
-  exact ha
-
 inductive Even : Nat → Prop
 | zero : Even Nat.zero
 | add_two : ∀ k : Nat, Even k → Even (k+2)
 | combine_two (n : Nat) (hn : Even n) : ∀ m : Nat, Even m → Even (n + m)
 
--- example (n : Nat) (h : Even n): Even (n + 2) := by
---   structured repeat apply Even.add_two _ _
---   exact h
-
--- example (n : Nat) : n = n := by
---   structured induction n
---   admit
-
-
-example (h : α ∧ β) : α ∨ b := by
-  structured 
-    have ha : α := h.left
-    have hb : β := h.right    
-  apply Or.intro_left _ ha
-
-example (n : Nat) : n = n := by
-  structured cases n
-  cases n with
-  | zero =>
-    show Nat.zero = Nat.zero
-
-    sorry
-  | succ n_1 =>
-    show (n_1 : Nat) ⊢ Nat.succ n_1 = Nat.succ n_1
-    sorry
-  -- cases n with
-  -- | zero => rfl
-  -- | succ m => rfl
-  -- repeat rfl
-
-example (n : Nat) (h : Even n) : Even (n + n + 2) := by
-  structured induction h
-  induction h with
-  | zero =>
-    show Even (Nat.zero + Nat.zero + 2)
-    sorry
-  | add_two k a a.ih =>
-    show (k : Nat) (a : Even k) (a.ih : Even (k + k + 2)) ⊢ Even (k + 2 + (k + 2) + 2)
-    sorry
-  | combine_two n_1 hn m a hn.ih a.ih =>
-    show (n_1 : Nat) (hn : Even n_1) (m : Nat) (a : Even m) (hn.ih : Even (n_1 + n_1 + 2)) 
-      (a.ih : Even (m + m + 2)) ⊢ Even (n_1 + m + (n_1 + m) + 2)
-    sorry
-  repeat admit
-
-
-  -- OR 
-  -- cases h
-  -- case zero =>
-  --   note ⊢ Even (Nat.zero + Nat.zero + 2)
-  --   sorry
-  -- case add_two k hk =>
-  --   note (k : Nat) (hk : Even k) ⊢ Even (k + 2 + (k + 2) + 2)
-  --   sorry
-  -- case combine_two k1 hk1 k2 hk2 => 
-  --   note (k1 : Nat) (hk1 : Even k1) (k2 : Nat) (hk2 : Even k2) ⊢ Even (k1 + k2 + (k1 + k2) + 2)
-  --   sorry
-  
-  -- In case of induction, for each inductive type, we have to add some `ih` to the end of args
-  -- induction h
-  -- case combine_two k1 k2 hk1 hk2 ih1 ih2 => 
-
-
-
-example (n : Nat) : α ↔ β := by
-  structured 
-    apply Iff.intro
-    intro _
-  case mp => admit
-  repeat admit
-
-  -- apply Iff.intro
-  -- case mp =>
-  --   note ⊢ α → β
-  --   sorry
-  -- case mpr =>
-  --   note ⊢ β → α
-  --   sorry
-
 example (n : Nat) : n = n := by
   structured 
-    -- TODO: Make inaccessible name an underscore in show, omit assertion ?
-    -- TODO TODO
-    -- TODO: still weird name _uniq.num
-    -- TODO: annotation doesn't change with case suggestion
     cases n
-    have _ : True := sorry
     try apply Even.zero
-  repeat admit
+  repeat sorry
 
 example : α ∧ β → β := by
-  -- structured intro (⟨ha, hb⟩) 
-  
-  note (ha : α) (hb : β) ⊢ β by intro (⟨ha, hb⟩)
-  sorry
+  structured intro ⟨_, _⟩ 
 
-#check LocalContext
+-- TODO: Wrap defaultCases in a show .. by .. block ?
